\documentclass[12pt]{article}   % you have 10pt, 11pt, or 12pt options

\include{header}

\title{LaTeX \, Template and Tutorial for Math Modelers}
\author{Not Me}
\date{\today}

\begin{document}

\section{Aufgabe 110}

$f \in C^1(\R^n, \R)$

$f(x + t_{min}) = \min\{f(x+td) : t \geq 0\}$

Wohldef: Sei m = $\inf\{f(x+td) : t \geq 0 \}$ 
\newline$\Rightarrow\exists$ Folge $(f(x+t_nd))_{n\in\N} \to m$
\\$(x+t_nd)_{n\in\N}$ Folge in $\mathcal{L}(x^{(0)})$, $\mathcal{L}(x^{(0)})$ kompakt
\newline$\Rightarrow\exists$ konvergente Teilfolge $(x+t_{n_k})_{k\in\N}\to x^*$

$f(x^*)$ = $\lim_{n \to \infty} f(x+t_{n_k}d) = \lim_{n\to\infty}f(x+t_nd) = m$
%$f(x^*)$ = $\lim\limits_{n \to \infty}$ \newline
%$f(x^*)$ = \[\lim_{n \to \infty}\]\newline

Mitten in anderer Aufgabe
$\min f(x)$ mit $f(x) = \frac12 x^TQx-c^Tx$, Q pos. def., $x^*$ lok. min

$\frac{f(x^k-\beta^{l_{k-1}}d^k)}{\beta^{l_{k-1}}}$

$\alpha\beta\beta\gamma\delta\epsilon\theta$

Aufgabe 122
$H^{(k)}$


zz. $d^{(k)}$ gradientenähnlich

\begin{gather}
	\norm{d^{(k)}} = \norm{-(H^{(k)})^{-1}  \nabla f(x^{(k)})} \leq \norm{-(H^{(k)})^{-1}} \norm{\nabla f(x^{(k)})} \leq \frac 1{\mu_1} \norm{\nabla f(x^{(k)})} \leq C  \\
-\nabla f(x^{(k_t)})^T(H^{(k)})^{-1}\nabla f(x^{(k_t)}) \leq -\frac 1{\mu_2}\norm{\nabla f(x^{(k_t)})} \leq -\varepsilon
\end{gather}

\vspace{3cm}
Aufgabe 124

a) $Q \in \R^{n\times n}, Q > 0, 0 < \lambda_1 \leq \lambda_2 \leq ... \leq \lambda_n$

\begin{gather}
	\lambda_1 \leq \frac{x^TQx}{x^Tx} \leq \lambda_n
\end{gather}
b) Für $x\in\R^n$ gilt:
\begin{align}
	f(x)-f(x^*) &= \frac12x^TQx+x^Tx-\frac12{x^*}^TQx^*-c^tx^* \\
	&= \frac12({x^*}^TQx+x^*Qx^*-2{x^*}^TQx^*+2{x^*}^TQx^*) + c^T(x-x^*) \\
	&= \frac12(x-x^*)^TQ(x-x^*) - {x^*}^TQx^*+x^TQx^*+(x-x^*)^Tc \\
	&= \frac12(x-x^*)^TQ(x-x^*)+ (x-x^*)^T(Qx^*+x)
\end{align}



123)
$f \in C^1(\R^n, \R)$, koerziv: Falls ${t^k}$, $\norm{z^k} \overset{k\to\infty}{\to}{test} \infty $, \newline
$\implies$
\blindtext

$a > 0 \land b > 0 \implies \frac ab > 0$

[Lemma 6.1]

$f:\R^n\to\R, (x^{(k)})_{k\in\N} \to x \in \R^n, (d^{(k)})_{k\in\N} \to d \in \R^n, (t_k)_{k\in\N} \to 0 \in R$ \\
$\implies \underset{k\to\infty}{\lim} \frac{f(x^{(k)}+t_kd^{(k)}) - f(x^{(k)})}{t_k} = \nabla {f(x)}^Td$


\end{document}
